matching-logic/src/Pattern.v
@@ -1057,3 +1057,60 @@ Proof.
   intros x. reflexivity.
 Defined.
 
+Lemma map_wf :
+  forall {Σ : Signature} (f : Pattern -> Pattern) l,
+    wf l -> (forall p, well_formed p -> well_formed (f p)) ->
+    wf (map f l).
+Proof.
+  induction l; intros; try by cbn in *.
+  cbn in *.
+  destruct_and!. apply H0 in H1.
+  specialize (IHl H2 H0). unfold wf in IHl.
+  by rewrite H1 IHl.
+Qed.
+
+Section corollaries.
+  Context {Σ : Signature}.
+
+  Lemma Forall_wf_map {A} (t : A -> Pattern) l : Forall (well_formed ∘ t) l <-> wf (map t l).
+  Proof.
+    intros. etransitivity. apply Forall_fold_right. unfold wf.
+    rewrite -> 2 foldr_map, foldr_andb_equiv_foldr_conj.
+    reflexivity.
+  Qed.
+
+  Corollary wf_fold_left {A : Type} (f : Pattern -> A -> Pattern) (t : A -> Pattern) x xs :
+    well_formed x ->
+    wf (map t xs) ->
+    (forall a b, well_formed a -> well_formed (t b) -> well_formed (f a b)) ->
+    well_formed (fold_left f xs x).
+  Proof.
+    intros. apply fold_left_ind with (Q := well_formed ∘ t);
+    only 2: apply Forall_wf_map; auto.
+  Defined.
+
+  Corollary wf_foldr {A : Type} (f : A -> Pattern -> Pattern) (t : A -> Pattern) x xs :
+    well_formed x ->
+    wf (map t xs) ->
+    (forall a b, well_formed a -> well_formed (t b) -> well_formed (f b a)) ->
+    well_formed (foldr f x xs).
+  Proof.
+    intros.
+    apply foldr_ind with (Q := well_formed ∘ t);
+    only 2: apply Forall_wf_map; auto.
+  Qed.
+
+  Corollary mf_fold_left {A : Type} (f : Pattern -> A -> Pattern) (t : A -> Pattern) x xs :
+    mu_free x ->
+    foldr (fun c a => mu_free c && a) true (map t xs) ->
+    (forall a b, mu_free a -> mu_free (t b) -> mu_free (f a b)) ->
+    mu_free (fold_left f xs x).
+  Proof.
+    intros.
+    apply fold_left_ind with (Q := mu_free ∘ t);
+    only 2: apply Forall_fold_right;
+    only 2: rewrite -> foldr_map, foldr_andb_equiv_foldr_conj in H0;
+    auto.
+  Qed.
+
+End corollaries.
